wip

LeanSubst/Basic.lean
@@ -1,15 +1,13 @@
 
 import Lean.Elab.Term
+import Lean.Elab.SyntheticMVars
 import Lilac
 open Lilac
 
 namespace LeanSubst
 
-universe u
-
 universe u1 u2 u3
 variable {S : Type u1} {T : Type u2} {U : Type u3}
-variable {V : List (Type u1)}
 
 namespace Subst.Syntax
   open Lean.Elab.Term
@@ -36,18 +34,18 @@ namespace Subst.Syntax
     | _ => Lean.Elab.throwUnsupportedSyntax
 end Subst.Syntax
 
-set_option linter.unusedVariables false in
-abbrev Var (T : Type u2) := Nat
-
-structure Ren (T : Type u2) where
-  act : Var T -> Var T
-
-@[simp]
+@[implicit_reducible, simp]
 def List.Tuple (F : Type u1 -> Type u2) : List (Type u1) -> Type u2
 | [] => ULift Unit
 | .cons x xs => F x × List.Tuple F xs
 
-class RenMap (S : Type u) (V : List (Type u)) where
+set_option linter.unusedVariables false in
+abbrev Var (T : Type u2) := Nat
+
+structure Ren (T : Type u2) where
+  act : Nat -> Nat
+
+class RenMap (S : Type u1) (V : List (Type u2)) where
   rmap : List.Tuple Ren V -> S -> S
 
 export RenMap (rmap)
@@ -60,7 +58,7 @@ open Lean.Elab.Term in
 open Subst.Syntax in
 elab_rules <= expected
 | `($t⟨ $elems,* ⟩) => do
-  let elems <- List.mapM id $ elems.getElems.foldl (λ acc t => elabTerm t none :: acc) []
+  let elems <- List.mapM id $ elems.getElems.foldl (λ acc t => elabTermAndSynthesize t none :: acc) []
   let elems_ty <- List.mapM id $ elems.map inferType |> List.map MetaM.promote |> List.map get_ty_arg
   let list_ann <- form_list elems_ty.reverse
   let elems_stx <- form_prod elems.reverse
@@ -70,20 +68,21 @@ elab_rules <= expected
 
 @[app_unexpander rmap]
 def unexpand_rmap : Lean.PrettyPrinter.Unexpander
+| `($_ ($r1, {down := ()}) $t) => `($t⟨$r1⟩)
 | `($_ ($r1, $r2, {down := ()}) $t) => `($t⟨$r1, $r2⟩)
 | `($_ ($r1, $r2, $r3, {down := ()}) $t) => `($t⟨$r1, $r2, $r3⟩)
 | `($_ $r $t) => `($t⟨$r,⟩)
 | _ => throw ()
 
 inductive Action (T : Type u2) where
-| re : Var T -> Action T
+| re : Nat -> Action T
 | su : T -> Action T
 deriving Repr
 
 export Action (re su)
 
 structure Subst (T : Type u2) where
-  inner : Var T -> Action T
+  inner : Nat -> Action T
 
 class SubstAction (T : Type u1) (A : Type u2) (U : outParam (Type u3)) where
   act (σ : Subst T) : A -> U
@@ -93,7 +92,7 @@ def Subst.act [SubstAction S T U] (σ : Subst S) : T -> U := SubstAction.act σ
 instance : SubstAction T Nat (Action T) where
   act := Subst.inner
 
-class SubstMap (S : Type u2) (V : List (Type u2)) where
+class SubstMap (S : Type u1) (V : List (Type u2)) where
   smap : List.Tuple Subst V -> S -> S
 
 export SubstMap (smap)
@@ -106,7 +105,7 @@ open Lean.Elab.Term in
 open Subst.Syntax in
 elab_rules <= expected
 | `($t[ $elems,* ]) => do
-  let elems <- List.mapM id $ elems.getElems.foldl (λ acc t => elabTerm t none :: acc) []
+  let elems <- List.mapM id $ elems.getElems.foldl (λ acc t => elabTermAndSynthesize t none :: acc) []
   let elems_ty <- List.mapM id $ elems.map inferType |> List.map MetaM.promote |> List.map get_ty_arg
   let list_ann <- form_list elems_ty.reverse
   let elems_stx <- form_prod elems.reverse
@@ -116,25 +115,10 @@ elab_rules <= expected
 
 @[app_unexpander smap]
 def unexpand_smap : Lean.PrettyPrinter.Unexpander
+| `($_ ($σ1, {down := ()}) $t) => `($t[$σ1])
 | `($_ ($σ1, $σ2, {down := ()}) $t) => `($t[$σ1, $σ2])
 | `($_ ($σ1, $σ2, $σ3, {down := ()}) $t) => `($t[$σ1, $σ2, $σ3])
 | `($_ $σ $t) => `($t[$σ,])
 | _ => throw ()
-
-
-def test1 : Subst Nat × ULift Unit -> Nat -> Nat := sorry
-
-instance : SubstMap Nat [Nat] where
-  smap := test1
-
-def test2 : Subst Nat × Subst Bool × ULift Unit -> Nat -> Nat := sorry
-
-instance : SubstMap Nat [Nat, Bool] where
-  smap := test2
-
-theorem test3 {r1 : Subst Nat} {r2 : Subst Bool} {x : Nat} : x[r1, r2] = x := sorry
-
-theorem test4 [SubstMap S V] {v : List.Tuple Subst V} {x : S} : x[v,] = x := sorry
-
 
 end LeanSubst
