LeanSubst/Class.lean
@@ -6,112 +6,128 @@ open Lilac
 namespace LeanSubst
 
 universe u1 u2 u3
-variable {S : Type u1} {T : Type u2} {U : Type u3}
-variable {n : Nat} {V : Vec (Type u2) n}
+variable {S : Type u1} {T T1 T2 : Type u2} {U : Type u3}
+variable {V : List (Type u2)}
 
-class RenMapId (S : Type u1) (T : Type u2) [RenMap S V] where
-  apply_id {s : S} : s⟨Ren.id T⟩ = s
+class RenMapId (S : Type u1) (V : List (Type u2)) [RenMap S V] where
+  apply_id {s : S} : s⟨Ren.ids V,⟩ = s
 
-class RenMapCompose (S : Type u1) (T : Type u2) [RenMap S T] where
-  apply_compose {s : S} {r1 r2 : Ren T} : s⟨r1⟩⟨r2⟩ = s⟨r1 ∘ r2⟩
+class RenMapCompose (S : Type u1) (V : List (Type u2)) [RenMap S V] where
+  apply_compose {s : S} {r1 r2 : List.Tuple Ren V} : s⟨r1,⟩⟨r2,⟩ = s⟨r1 ∘ r2,⟩
 
 @[simp]
-theorem Ren.apply_id [RenMap S T] [RenMapId S T] {s : S} : s⟨id T⟩ = s := RenMapId.apply_id
+theorem Ren.apply_id [RenMap S V] [RenMapId S V] {s : S} : s⟨ids V,⟩ = s := RenMapId.apply_id
+
+@[simp]
+theorem Ren.apply_id1 [RenMap S [T]] [RenMapId S [T]] {s : S} : s⟨id T⟩ = s := RenMapId.apply_id
+
+@[simp]
+theorem Ren.apply_id2 [RenMap S [T1, T2]] [RenMapId S [T1, T2]] {s : S} : s⟨id T1, id T2⟩ = s := RenMapId.apply_id
 
 @[simp, grind =]
-theorem Ren.apply_compose [RenMap S T] [RenMapCompose S T] {s : S} {r1 r2 : Ren T}
-  : s⟨r1⟩⟨r2⟩ = s⟨r1 ∘ r2⟩
+theorem Ren.apply_compose [RenMap S V] [RenMapCompose S V] {s : S} {r1 r2 : List.Tuple Ren V}
+  : s⟨r1,⟩⟨r2,⟩ = s⟨r1 ∘ r2,⟩
 := RenMapCompose.apply_compose
 
-instance (priority := high) [RenMap T T] [RenMapId T T] : RenMapId (Action T) T where
-  apply_id := by intro s; cases s <;> simp
+instance : RenMap Nat [Nat, Bool] where
+  rmap := sorry
 
-instance [RenMap S T] [RenMapId S T] : RenMapId (Action S) T where
-  apply_id := by intro s; cases s <;> simp
+instance : RenMapId Nat [Nat, Bool] where
+  apply_id := sorry
 
-instance (priority := high) [RenMap T T] [RenMapCompose T T] : RenMapCompose (Action T) T where
-  apply_compose := by intro s; cases s <;> simp
+theorem test1 (x : Nat) : x⟨Ren.id Nat, Ren.id Bool⟩ = x := by
+  simp
+  sorry
 
-instance [RenMap S T] [RenMapCompose S T] : RenMapCompose (Action S) T where
-  apply_compose := by intro s; cases s <;> simp
+-- instance (priority := high) [RenMap T T] [RenMapId T T] : RenMapId (Action T) T where
+--   apply_id := by intro s; cases s <;> simp
 
-class SubstMapStable (S : Type u1) (T : Type u2) [RenMap S T] [SubstMap S T] where
-  apply_stable (r : Ren T) (σ : Subst T) : r.to = σ -> rmap (S := S) r = smap σ
+-- instance [RenMap S T] [RenMapId S T] : RenMapId (Action S) T where
+--   apply_id := by intro s; cases s <;> simp
 
-class SubstMapId (S : Type u1) (T : Type u2) [SubstMap S T] where
-  apply_id {s : S} : s[.id T] = s
+-- instance (priority := high) [RenMap T T] [RenMapCompose T T] : RenMapCompose (Action T) T where
+--   apply_compose := by intro s; cases s <;> simp
 
-class SubstMapRenComposeLeft (S : Type u1) (T : Type u2) [RenMap S T] [SubstMap S T] where
-  apply_ren_compose_left {s : S} {r : Ren T} {τ : Subst T} : s⟨r⟩[τ] = s[r ∘ τ]
+-- instance [RenMap S T] [RenMapCompose S T] : RenMapCompose (Action S) T where
+--   apply_compose := by intro s; cases s <;> simp
 
-class SubstMapRenComposeRight (S : Type u1) (T : Type u2) [RenMap S T] [RenMap T T] [SubstMap S T] where
-  apply_ren_compose_right {s : S} {r : Ren T} {σ : Subst T} : s[σ]⟨r⟩ = s[σ ∘ r]
+-- class SubstMapStable (S : Type u1) (T : Type u2) [RenMap S T] [SubstMap S T] where
+--   apply_stable (r : Ren T) (σ : Subst T) : r.to = σ -> rmap (S := S) r = smap σ
 
-class SubstMapCompose (S : Type u1) (T : Type u2) [SubstMap S T] [SubstMap T T] where
-  apply_compose {s : S} {σ τ : Subst T} : s[σ][τ] = s[σ ∘ τ]
+-- class SubstMapId (S : Type u1) (T : Type u2) [SubstMap S T] where
+--   apply_id {s : S} : s[.id T] = s
 
-class SubstMapRenCommute (S : Type u1) (T : Type u2) [RenMap S S] [RenMap S T] [SubstMap S T] where
-  apply_commute_ren_subst {s : S} {r : Ren S} {τ : Subst T} : s⟨r⟩[τ] = s[τ]⟨r⟩
-  apply_commute_ren_ren {s : S} {r1 : Ren S} {r2 : Ren T} : s⟨r1⟩⟨r2⟩ = s⟨r2⟩⟨r1⟩
+-- class SubstMapRenComposeLeft (S : Type u1) (T : Type u2) [RenMap S T] [SubstMap S T] where
+--   apply_ren_compose_left {s : S} {r : Ren T} {τ : Subst T} : s⟨r⟩[τ] = s[r ∘ τ]
 
-class SubstMapRenHetCompose (S : Type u1) (T : Type u2) [RenMap S T] [SubstMap S S] where
-  apply_hcompose_ren {s : S} {σ : Subst S} {r : Ren T} : s[σ]⟨r⟩ = s⟨r⟩[σ ◾ r]
+-- class SubstMapRenComposeRight (S : Type u1) (T : Type u2) [RenMap S T] [RenMap T T] [SubstMap S T] where
+--   apply_ren_compose_right {s : S} {r : Ren T} {σ : Subst T} : s[σ]⟨r⟩ = s[σ ∘ r]
 
-class SubstMapHetCompose (S : Type u1) (T : Type u2) [SubstMap S S] [SubstMap S T] where
-  apply_hcompose {s : S} {σ : Subst S} {τ : Subst T} : s[σ][τ] = s[τ][σ ◾ τ]
+-- class SubstMapCompose (S : Type u1) (T : Type u2) [SubstMap S T] [SubstMap T T] where
+--   apply_compose {s : S} {σ τ : Subst T} : s[σ][τ] = s[σ ∘ τ]
 
-theorem Subst.apply_stable
-  [RenMap S T] [SubstMap S T] [SubstMapStable S T]
-  {r : Ren T} {σ : Subst T}
-  : r.to = σ -> rmap (S := S) r = smap σ
-:= SubstMapStable.apply_stable _ _
+-- class SubstMapRenCommute (S : Type u1) (T : Type u2) [RenMap S S] [RenMap S T] [SubstMap S T] where
+--   apply_commute_ren_subst {s : S} {r : Ren S} {τ : Subst T} : s⟨r⟩[τ] = s[τ]⟨r⟩
+--   apply_commute_ren_ren {s : S} {r1 : Ren S} {r2 : Ren T} : s⟨r1⟩⟨r2⟩ = s⟨r2⟩⟨r1⟩
 
-@[simp, grind =]
-theorem Subst.apply_id [SubstMap S T] [SubstMapId S T] {s : S} : s[.id T] = s := SubstMapId.apply_id
+-- class SubstMapRenHetCompose (S : Type u1) (T : Type u2) [RenMap S T] [SubstMap S S] where
+--   apply_hcompose_ren {s : S} {σ : Subst S} {r : Ren T} : s[σ]⟨r⟩ = s⟨r⟩[σ ◾ r]
 
-@[simp, grind =]
-theorem Subst.apply_ren_compose_left [RenMap S T] [SubstMap S T] [SubstMapRenComposeLeft S T]
-  {s : S} {r : Ren T} {τ : Subst T}
-  : s⟨r⟩[τ] = s[r ∘ τ]
-:= SubstMapRenComposeLeft.apply_ren_compose_left
+-- class SubstMapHetCompose (S : Type u1) (T : Type u2) [SubstMap S S] [SubstMap S T] where
+--   apply_hcompose {s : S} {σ : Subst S} {τ : Subst T} : s[σ][τ] = s[τ][σ ◾ τ]
 
-@[simp, grind =]
-theorem Subst.apply_ren_compose_right
-  [RenMap S T] [RenMap T T] [SubstMap S T] [SubstMapRenComposeRight S T]
-  {s : S} {σ : Subst T} {r : Ren T}
-  : s[σ]⟨r⟩ = s[σ ∘ r]
-:= SubstMapRenComposeRight.apply_ren_compose_right
+-- theorem Subst.apply_stable
+--   [RenMap S T] [SubstMap S T] [SubstMapStable S T]
+--   {r : Ren T} {σ : Subst T}
+--   : r.to = σ -> rmap (S := S) r = smap σ
+-- := SubstMapStable.apply_stable _ _
 
-@[grind =]
-theorem Subst.apply_commute_ren_subst
-  [RenMap S S] [RenMap S T] [SubstMap S T] [SubstMapRenCommute S T]
-  {s : S} {r : Ren S} {τ : Subst T}
-  : s⟨r⟩[τ] = s[τ]⟨r⟩
-:= SubstMapRenCommute.apply_commute_ren_subst
+-- @[simp, grind =]
+-- theorem Subst.apply_id [SubstMap S T] [SubstMapId S T] {s : S} : s[.id T] = s := SubstMapId.apply_id
 
-@[grind =]
-theorem Subst.apply_commute_ren_ren
-  [RenMap S S] [RenMap S T] [SubstMap S T] [SubstMapRenCommute S T]
-  {s : S} {r1 : Ren S} {r2 : Ren T}
-  : s⟨r1⟩⟨r2⟩ = s⟨r2⟩⟨r1⟩
-:= SubstMapRenCommute.apply_commute_ren_ren
+-- @[simp, grind =]
+-- theorem Subst.apply_ren_compose_left [RenMap S T] [SubstMap S T] [SubstMapRenComposeLeft S T]
+--   {s : S} {r : Ren T} {τ : Subst T}
+--   : s⟨r⟩[τ] = s[r ∘ τ]
+-- := SubstMapRenComposeLeft.apply_ren_compose_left
 
-@[simp, grind =]
-theorem Subst.apply_compose [SubstMap S T] [SubstMap T T] [SubstMapCompose S T]
-  {s : S} {σ τ : Subst T}
-  : s[σ][τ] = s[σ ∘ τ]
-:= SubstMapCompose.apply_compose
+-- @[simp, grind =]
+-- theorem Subst.apply_ren_compose_right
+--   [RenMap S T] [RenMap T T] [SubstMap S T] [SubstMapRenComposeRight S T]
+--   {s : S} {σ : Subst T} {r : Ren T}
+--   : s[σ]⟨r⟩ = s[σ ∘ r]
+-- := SubstMapRenComposeRight.apply_ren_compose_right
 
-@[simp, grind =]
-theorem Subst.apply_hcompose_ren [SubstMap S S] [RenMap S T] [SubstMapRenHetCompose S T]
-  {s : S} {σ : Subst S} {r : Ren T}
-  : s[σ]⟨r⟩ = s⟨r⟩[σ ◾ r]
-:= SubstMapRenHetCompose.apply_hcompose_ren
+-- @[grind =]
+-- theorem Subst.apply_commute_ren_subst
+--   [RenMap S S] [RenMap S T] [SubstMap S T] [SubstMapRenCommute S T]
+--   {s : S} {r : Ren S} {τ : Subst T}
+--   : s⟨r⟩[τ] = s[τ]⟨r⟩
+-- := SubstMapRenCommute.apply_commute_ren_subst
 
-@[simp, grind =]
-theorem Subst.apply_hcompose [SubstMap S S] [SubstMap S T] [SubstMapHetCompose S T]
-  {s : S} {σ : Subst S} {τ : Subst T}
-  : s[σ][τ] = s[τ][σ ◾ τ]
-:= SubstMapHetCompose.apply_hcompose
+-- @[grind =]
+-- theorem Subst.apply_commute_ren_ren
+--   [RenMap S S] [RenMap S T] [SubstMap S T] [SubstMapRenCommute S T]
+--   {s : S} {r1 : Ren S} {r2 : Ren T}
+--   : s⟨r1⟩⟨r2⟩ = s⟨r2⟩⟨r1⟩
+-- := SubstMapRenCommute.apply_commute_ren_ren
+
+-- @[simp, grind =]
+-- theorem Subst.apply_compose [SubstMap S T] [SubstMap T T] [SubstMapCompose S T]
+--   {s : S} {σ τ : Subst T}
+--   : s[σ][τ] = s[σ ∘ τ]
+-- := SubstMapCompose.apply_compose
+
+-- @[simp, grind =]
+-- theorem Subst.apply_hcompose_ren [SubstMap S S] [RenMap S T] [SubstMapRenHetCompose S T]
+--   {s : S} {σ : Subst S} {r : Ren T}
+--   : s[σ]⟨r⟩ = s⟨r⟩[σ ◾ r]
+-- := SubstMapRenHetCompose.apply_hcompose_ren
+
+-- @[simp, grind =]
+-- theorem Subst.apply_hcompose [SubstMap S S] [SubstMap S T] [SubstMapHetCompose S T]
+--   {s : S} {σ : Subst S} {τ : Subst T}
+--   : s[σ][τ] = s[τ][σ ◾ τ]
+-- := SubstMapHetCompose.apply_hcompose
 
 end LeanSubst
